theories/case_studies/lse_downward/lse.v
@@ -1,0 +1,122 @@
+From iris.algebra Require Import frac.
+From iris.proofmode Require Import proofmode.
+From cap_machine Require Import rules proofmode.
+From cap_machine Require Import fetch assert switcher.
+
+Section LSE_Main.
+  Context `{MP: MachineParameters}.
+
+  (** CHERIoT code for the LSE downward example
+
+      ```
+int a = 2;
+
+void __cheri_compartment("known") f(void)
+{
+  int *y;             // allocate an address on top of the stack frame
+  *y = &a;            // push the (global) capability pointing to `a` on top of the stack frame
+  assert ( a == 2 );  // check the integrity of `a`
+	return;
+}
+
+int __cheri_compartment("known") run()
+{
+	// call unknown program
+	adv();
+	return 0;
+}
+      ```
+
+   *)
+
+  (** The LSE downward example relies on protection against dangling pointers.
+      In short, a global capability points-to the CGP address `a` and contains 2.
+      The function `f` ( a closure ) pushes the capability on top of the stack,
+      and checks integrity of `a` (ie., it contains 2).
+
+      The correctness of the example relies on the fact that,
+      when `f` returns, its stack frame is popped
+      (in CHERIoT, understand cleared by the switcher)
+      and the content is not accessible by the caller anymore.
+   *)
+
+  (*
+    PSEUDO-CODE:
+
+    run:
+      set a := 2
+      call B.adv
+      halt
+
+    f:
+      push (RW, Global, a, a+1, a)
+      assert (a == 2)
+      return
+   *)
+
+  Definition LSE_main_code_run : list Word :=
+    (* set a := 2 *)
+    encodeInstrsW [
+        Store cgp 2
+      ]
+    (* call B.adv LSE.awkward *)
+    ++ fetch_instrs 0 ct0 cs0 cs1 (* ct0 -> switcher entry point *)
+    ++ fetch_instrs 2 ct1 cs0 cs1 (* ct1 -> {B.adv}_(ot_switcher)  *)
+    ++
+    encodeInstrsW [
+      Jalr cra ct0; (* jmp to entry point *)
+      Halt
+    ].
+
+  Definition LSE_main_code_f : list Word :=
+    (* push a := (RW, Global, a, a+1, a) *)
+    encodeInstrsW [
+        GetB cs0 cgp;
+        machine_base.Add cs1 cs0 1;
+        Subseg cgp cs0 cs1; (* cgp := (RW, Global, a, a+1, a) *)
+        (* csp = (RWL, Local, bstk, estk, bstk)  *)
+        Store csp cgp; (* bstk -> (RW, Global, a, a+1, a) *)
+        (* -- assert (a == 2) -- *)
+        Load ct0 cgp;
+        Mov ct1 2
+      ]
+      ++ assert_instrs 1 cgp cs0 cs1 (* asserts that ( *ct0 = *ct1 ) *)
+      ++ encodeInstrsW [
+        (* return 0 *)
+        Mov ca0 0%Z;
+        Mov ca1 0%Z;
+        JmpCap cra
+      ].
+
+  Definition lse_main_code : list Word
+    := LSE_main_code_run ++ LSE_main_code_f.
+
+  Definition lse_main_data : list Word := [WInt 2].
+
+  Definition lse_main_imports
+    (b_switcher e_switcher a_cc_switcher : Addr) (ot_switcher : OType)
+    (b_assert e_assert : Addr)
+    (B_adv : Sealable)
+    : list Word :=
+    [
+      WSentry XSRW_ Local b_switcher e_switcher a_cc_switcher;
+      WSentry RX Global b_assert e_assert b_assert;
+      WSealed ot_switcher B_adv
+    ].
+
+  Definition length_lse_main_imports :=
+    length
+      (lse_main_imports za za za za_ot za za (SCap RO Global za za za)).
+
+  Definition lse_exp_tbl_entry_f :=
+    WInt (encode_entry_point 0
+            (length_lse_main_imports + (length LSE_main_code_run))).
+
+  Definition lse_entry_f_sb
+    b_lse_exp_tbl e_lse_exp_tbl : Sealable :=
+      SCap RO Global b_lse_exp_tbl e_lse_exp_tbl (b_lse_exp_tbl ^+2)%a.
+
+  Definition lse_export_table_entries : list Word :=
+    [ lse_exp_tbl_entry_f ].
+
+End LSE_Main.
