theories/case_studies/lse_downward/lse_spec.v
@@ -1,0 +1,297 @@
+From iris.proofmode Require Import proofmode.
+From cap_machine Require Import region_invariants_revocation interp_weakening monotone.
+From cap_machine Require Import rules logrel logrel_extra monotone proofmode register_tactics.
+From cap_machine Require Import fetch assert switcher switcher_spec_call.
+From cap_machine Require Import lse lse_spec_closure.
+From cap_machine Require Import proofmode.
+
+Section LSE.
+  Context
+    {Σ:gFunctors}
+    {ceriseg:ceriseG Σ} {sealsg: sealStoreG Σ}
+    {Cname : CmptNameG}
+    {stsg : STSG Addr region_type Σ} {heapg : heapGS Σ}
+    {nainv: logrel_na_invs Σ}
+    {cstackg : CSTACKG Σ}
+    `{MP: MachineParameters}
+    {swlayout : switcherLayout}
+  .
+
+  Context {C : CmptName}.
+
+  Implicit Types W : WORLD.
+  Implicit Types C : CmptName.
+  Notation V := (WORLD -n> (leibnizO CmptName) -n> (leibnizO Word) -n> iPropO Σ).
+
+  Lemma lse_run_spec
+
+    (pc_b pc_e pc_a : Addr)
+    (cgp_b cgp_e : Addr)
+    (csp_b csp_e : Addr)
+    (rmap : Reg)
+
+    (b_lse_exp_tbl e_lse_exp_tbl : Addr)
+
+    (b_assert e_assert : Addr) (a_flag : Addr)
+    (C_f : Sealable)
+
+    (W0 : WORLD)
+
+    (Ws : list WORLD)
+    (Cs : list CmptName)
+
+    (Nassert Nswitcher Nlse_code LSEN : namespace)
+
+    (cstk : CSTK)
+    :
+
+    let imports :=
+     lse_main_imports
+       b_switcher e_switcher a_switcher_call ot_switcher b_assert e_assert C_f
+    in
+
+    Nswitcher ## Nassert ->
+    Nswitcher ## Nlse_code ->
+    Nassert ## Nlse_code ->
+
+    (b_lse_exp_tbl <= b_lse_exp_tbl ^+ 2 < e_lse_exp_tbl)%a ->
+
+    dom rmap = all_registers_s ∖ {[ PC ; cgp ; csp]} ->
+    (forall r, r ∈ (dom rmap) -> is_Some (rmap !! r) ) ->
+    SubBounds pc_b pc_e pc_a (pc_a ^+ length lse_main_code)%a ->
+
+    (cgp_b + length lse_main_data)%a = Some cgp_e ->
+    (pc_b + length imports)%a = Some pc_a ->
+
+    frame_match Ws Cs cstk W0 C ->
+    (
+      na_inv logrel_nais Nassert (assert_inv b_assert e_assert a_flag)
+      ∗ na_inv logrel_nais Nswitcher switcher_inv
+      ∗ na_inv logrel_nais LSEN
+          ([[ pc_b , pc_a ]] ↦ₐ [[ imports ]]
+           ∗ codefrag pc_a lse_main_code
+           ∗ cgp_b ↦ₐ WInt 2
+          )
+      ∗ inv (export_table_PCCN LSEN) (b_lse_exp_tbl ↦ₐ WCap RX Global pc_b pc_e pc_b)
+      ∗ inv (export_table_CGPN LSEN) ((b_lse_exp_tbl ^+ 1)%a ↦ₐ WCap RW Global cgp_b cgp_e cgp_b)
+      ∗ inv (export_table_entryN LSEN (b_lse_exp_tbl ^+ 2)%a)
+          ((b_lse_exp_tbl ^+ 2)%a ↦ₐ lse_exp_tbl_entry_f)
+      ∗ na_own logrel_nais ⊤
+
+      (* initial register file *)
+      ∗ PC ↦ᵣ WCap RX Global pc_b pc_e pc_a
+      ∗ cgp ↦ᵣ WCap RW Global cgp_b cgp_e cgp_b
+      ∗ csp ↦ᵣ WCap RWL Local csp_b csp_e csp_b
+      ∗ ( [∗ map] r↦w ∈ rmap, r ↦ᵣ w )
+
+      (* initial memory layout *)
+      ∗ region W0 C ∗ sts_full_world W0 C
+
+      ∗ interp_continuation cstk Ws Cs
+
+      ∗ cstack_frag cstk
+
+      ∗ interp W0 C (WSealed ot_switcher C_f)
+      ∗ (WSealed ot_switcher C_f) ↦□ₑ 0
+      ∗ interp W0 C (WCap RWL Local csp_b csp_e csp_b)
+
+      ∗ WSealed ot_switcher (SCap RO Global b_lse_exp_tbl e_lse_exp_tbl (b_lse_exp_tbl ^+ 2)%a) ↦□ₑ 0
+      ∗ WSealed ot_switcher (SCap RO Local b_lse_exp_tbl e_lse_exp_tbl (b_lse_exp_tbl ^+ 2)%a) ↦□ₑ 0
+      ∗ seal_pred ot_switcher ot_switcher_propC
+
+      ⊢ WP Seq (Instr Executable) {{ v, ⌜v = HaltedV⌝ → na_own logrel_nais ⊤ }})%I.
+  Proof.
+    intros imports; subst imports.
+    iIntros (HNswitcher_assert HNswitcher_lse HNassert_lse Hsize_lse_exp_tbl Hrmap_dom Hrmap_init HsubBounds
+               Hcgp_contiguous Himports_contiguous Hframe_match
+            )
+      "(#Hassert & #Hswitcher
+      & #Hlse
+      & #Hlse_exp_tbl_PCC
+      & #Hlse_exp_tbl_CGP
+      & #Hlse_exp_tbl_awkward
+      & Hna
+      & HPC & Hcgp & Hcsp & Hrmap
+      & Hr_C & Hsts_C
+      & HK
+      & Hcstk_frag
+      & #Hinterp_W0_C_f
+      & #HentryC_f
+      & #Hinterp_W0_csp
+      & #Hentry_f & #Hentry_f'
+      & #Hot_switcher
+      )".
+    iMod (na_inv_acc with "Hlse Hna")
+      as "(( >Himports_main & >Hcode_main & >Hcgp_b) & Hna & Hlse_close)"; auto.
+    codefrag_facts "Hcode_main"; rename H into Hpc_contiguous ; clear H0.
+    (* --- Extract registers ca0 ct0 ct1 ct2 ct3 cs0 cs1 --- *)
+    iExtractList "Hrmap" [cra;ct0;ct1;cs0;cs1]
+      as ["Hcra"; "Hct0"; "Hct1"; "Hcs0"; "Hcs1"].
+
+    (* Extract the imports *)
+    iDestruct (region_pointsto_cons with "Himports_main") as "[Himport_switcher Himports_main]".
+    { transitivity (Some (pc_b ^+ 1)%a); auto; solve_addr. }
+    { solve_addr. }
+    iDestruct (region_pointsto_cons with "Himports_main") as "[Himport_assert Himports_main]".
+    { transitivity (Some (pc_b ^+ 2)%a); auto; solve_addr. }
+    { solve_addr. }
+    iDestruct (region_pointsto_cons with "Himports_main") as "[Himport_C_f Himports_main]".
+    { transitivity (Some (pc_b ^+ 3)%a); auto; solve_addr. }
+    { solve_addr. }
+
+    (* Revoke the world to get the stack frame *)
+    set (stk_frame_addrs := finz.seq_between csp_b csp_e).
+    iAssert ([∗ list] a ∈ stk_frame_addrs, ⌜W0.1 !! a = Some Temporary⌝)%I as "Hstk_frm_tmp_W0".
+    { iApply (writeLocalAllowed_valid_cap_implies_full_cap with "Hinterp_W0_csp"); eauto. }
+
+    iMod (monotone_revoke_stack_alt with "[$Hinterp_W0_csp $Hsts_C $Hr_C]")
+        as (l) "(%Hl_unk & Hsts_C & Hr_C & Hfrm_close_W0 & >[%stk_mem Hstk] & Hrevoked_l)".
+    set (W1 := revoke W0).
+
+    (* --------------------------------------------------------------- *)
+    (* ----------------- Start the proof of the code ----------------- *)
+    (* --------------------------------------------------------------- *)
+
+    (* --------------------------------------------------- *)
+    (* ----------------- BLOCK 0 : INIT ------------------ *)
+    (* --------------------------------------------------- *)
+    rewrite /lse_main_code /LSE_main_code_run.
+    rewrite -!app_assoc.
+    focus_block_0 "Hcode_main" as "Hcode" "Hcont"; iHide "Hcont" as hcont.
+
+    (* Store cgp 0%Z; *)
+    iInstr "Hcode".
+    { apply withinBounds_true_iff; solve_addr. }
+    subst hcont; unfocus_block "Hcode" "Hcont" as "Hcode_main".
+
+    (* --------------------------------------------------- *)
+    (* -------------- BLOCK 1 to 3 : FETCH --------------- *)
+    (* --------------------------------------------------- *)
+
+    focus_block 1 "Hcode_main" as a_fetch1 Ha_fetch1 "Hcode" "Hcont"; iHide "Hcont" as hcont.
+    iApply (fetch_spec with "[- $HPC $Hct0 $Hcs0 $Hcs1 $Hcode]"); eauto.
+    { apply withinBounds_true_iff; solve_addr. }
+    replace (pc_b ^+ 0)%a with pc_b by solve_addr.
+    iFrame "Himport_switcher".
+    iNext ; iIntros "(HPC & Hct0 & Hcs0 & Hcs1 & Hcode & Himport_switcher)".
+    iEval (cbn) in "Hct0".
+    subst hcont; unfocus_block "Hcode" "Hcont" as "Hcode_main".
+
+    focus_block 2 "Hcode_main" as a_fetch2 Ha_fetch2 "Hcode" "Hcont"; iHide "Hcont" as hcont; clear dependent a_fetch1.
+    iApply (fetch_spec with "[- $HPC $Hct1 $Hcs0 $Hcs1 $Hcode $Himport_C_f]"); eauto.
+    { apply withinBounds_true_iff; solve_addr. }
+    iNext ; iIntros "(HPC & Hct1 & Hcs0 & Hcs1 & Hcode & Himport_C_f)".
+    iEval (cbn) in "Hct1".
+    subst hcont; unfocus_block "Hcode" "Hcont" as "Hcode_main".
+
+    (* --------------------------------------------------- *)
+    (* ----------------- BLOCK 3: CALL B ----------------- *)
+    (* --------------------------------------------------- *)
+
+    focus_block 3 "Hcode_main" as a_callB Ha_callB "Hcode" "Hcont"; iHide "Hcont" as hcont; clear dependent a_fetch2.
+    (* Jalr cra ct0; *)
+    iInstr "Hcode".
+
+
+    (*  -- prove that the LSE_awkward entry point is safe-to-share -- *)
+
+    (* -- separate argument registers -- *)
+    iExtractList "Hrmap" [ca0;ca1;ca2;ca3;ca4;ca5]
+      as ["Hca0"; "Hca1"; "Hca2"; "Hca3"; "Hca4"; "Hca5"].
+
+    set ( rmap_arg :=
+           {[ ca0 := wca0;
+              ca1 := wca1;
+              ca2 := wca2;
+              ca3 := wca3;
+              ca4 := wca4;
+              ca5 := wca5;
+              ct0 := WSentry XSRW_ Local b_switcher e_switcher a_switcher_call
+           ]} : Reg
+        ).
+
+    set (rmap' := (delete ca5 _)).
+
+    pose proof (revoke_related_sts_priv_world W0) as Hpriv_W0_W1.
+
+    (* Show that the entry point to C_f is still safe in W1 *)
+    iAssert (interp W1 C (WSealed ot_switcher C_f)) as "#Hinterp_W1_C_f".
+    { iApply interp_monotone_sd; eauto. }
+    iClear "Hinterp_W0_C_f".
+
+    (* Show that the arguments are safe, when necessary *)
+    iAssert ([∗ map] rarg↦warg ∈ rmap_arg, rarg ↦ᵣ warg
+                                           ∗ (if decide (rarg ∈ dom_arg_rmap 0)
+                                             then interp W1 C warg
+                                             else True)
+            )%I
+      with "[Hca0 Hca1 Hca2 Hca3 Hca4 Hca5 Hct0]" as "Hrmap_arg".
+    { subst rmap_arg.
+      repeat (iApply big_sepM_insert; [done|iFrame "∗#"]).
+      done.
+    }
+
+    (* Prepare the closing resources for the switcher call spec *)
+    iAssert (
+        ([∗ list] a ∈ finz.seq_between csp_b csp_e, closing_revoked_resources W1 C a ∗
+                                                    ⌜W1.1 !! a = Some Revoked⌝)
+      )%I with "[Hfrm_close_W0]" as "#Hfrm_close_W1".
+    {
+      iApply (big_sepL_impl with "Hfrm_close_W0").
+      iModIntro; iIntros (k a Ha) "[Hclose %Hrev]".
+      iDestruct (mono_priv_closing_revoked_resources with "Hclose") as "$"; auto.
+    }
+    subst hcont; unfocus_block "Hcode" "Hcont" as "Hcode_main".
+
+    iMod ("Hlse_close" with
+           "[$Hna Himport_assert Himport_switcher Himport_C_f Himports_main $Hcode_main $Hcgp_b]")
+      as "Hna".
+    { iNext.
+      iDestruct (region_pointsto_cons with "[$Himport_C_f $Himports_main]") as "Himports_main"
+      ; [solve_addr|solve_addr|].
+      iDestruct (region_pointsto_cons with "[$Himport_assert $Himports_main]") as "Himports_main"
+      ; [solve_addr|solve_addr|].
+      iDestruct (region_pointsto_cons with "[$Himport_switcher $Himports_main]") as "$" ;solve_addr.
+    }
+
+    (* Apply the spec switcher call *)
+    iApply (switcher_cc_specification with
+             "[- $Hswitcher $Hna
+              $HPC $Hcgp $Hcra $Hcsp $Hct1 $Hcs0 $Hcs1 $HentryC_f $Hrmap_arg $Hrmap
+              $Hstk $Hr_C $Hsts_C $Hfrm_close_W1 $Hcstk_frag
+              $Hinterp_W1_C_f $HK]"); eauto.
+    { subst rmap'.
+      repeat (rewrite dom_delete_L); repeat (rewrite dom_insert_L).
+      rewrite /dom_arg_rmap Hrmap_dom.
+      set_solver+.
+    }
+    { by rewrite /is_arg_rmap. }
+
+    clear dependent wct0 wct1 wcs0 wcs1.
+    clear dependent wca0 wca1 wca2 wca3 wca4 wca5 rmap.
+    iNext.
+    iIntros (W2 rmap stk_mem_l stk_mem_h)
+      "(%Hrelated_pub_W2ext_W2 & %Hdom_rmap
+      & Hna & #Hinterp_W2_csp & %Hcsp_bounds
+      & Hsts_C & Hr_C & Hfrm_close_W2
+      & Hcstk_frag & Hrel_stk_C
+      & HPC & Hcgp & Hcra & Hcs0 & Hcs1 & Hcsp
+      & [%warg0 [Hca0 _] ] & [%warg1 [Hca1 _] ]
+      & Hrmap & Hstk_l & Hstk_h & HK)".
+    iEval (cbn) in "HPC".
+
+    (* Halt *)
+    iMod (na_inv_acc with "Hlse Hna")
+      as "(( >Himports_main & >Hcode_main & >Hcgp_b) & Hna & Hlse_close)"; auto.
+    replace (encodeInstrsW [Jalr cra ct0; Halt]) with
+      (encodeInstrsW [Jalr cra ct0] ++ encodeInstrsW [Halt])
+    by auto.
+    rewrite -app_assoc.
+    focus_block 4 "Hcode_main" as a_callB' Ha_callB' "Hcode" "Hcont"; iHide "Hcont" as hcont.
+    iInstr "Hcode".
+    subst hcont; unfocus_block "Hcode" "Hcont" as "Hcode_main".
+    iMod ("Hlse_close" with "[$Hna $Himports_main $Hcode_main $Hcgp_b]") as "Hna".
+    wp_end; iIntros "_"; iFrame.
+  Qed.
+
+End LSE.
